Move helpers to SteelSelGhost effect

pulse/ulib/experimental/Steel.SelEffect.Atomic.fst
@@ -19,8 +19,6 @@ module Steel.SelEffect.Atomic
 open Steel.SelEffect
 friend Steel.SelEffect
 
-
-
 #set-options "--warn_error -330"  //turn off the experimental feature warning
 
 let _ : squash (forall (pre:pre_t) (m0:mem{interp (hp_of pre) m0}) (m1:mem{disjoint m0 m1}).
@@ -278,3 +276,363 @@ let bind_pure_steela_ a b opened o f g
 let lift_ghost_atomic a o f = f
 
 let lift_atomic_steel a o f = f
+
+(* Some helpers *)
+
+let get0 (#opened:inames) (#p:vprop) (_:unit) : repr (rmem p)
+  true opened Unobservable p (fun _ -> p)
+  (requires fun _ -> True)
+  (ensures fun h0 r h1 -> normal (frame_equalities p h0 h1 /\ frame_equalities p r h1))
+  = fun frame ->
+      let m0:full_mem = NMSTTotal.get () in
+      let h0 = mk_rmem p (core_mem m0) in
+      lemma_frame_equalities_refl p h0;
+      h0
+
+let get _ = SteelSelGhostF?.reflect (get0 ())
+
+let intro_star (p q:vprop) (r:slprop) (vp:erased (t_of p)) (vq:erased (t_of q)) (m:mem)
+  (proof:(m:mem) -> Lemma
+    (requires interp (hp_of p) m /\ sel_of p m == reveal vp)
+    (ensures interp (hp_of q) m)
+  )
+  : Lemma
+   (requires interp ((hp_of p) `Mem.star` r) m /\ sel_of p m == reveal vp)
+   (ensures interp ((hp_of q) `Mem.star` r) m)
+= let p = hp_of p in
+  let q = hp_of q in
+  let intro (ml mr:mem) : Lemma
+      (requires interp q ml /\ interp r mr /\ disjoint ml mr)
+      (ensures disjoint ml mr /\ interp (q `Mem.star` r) (Mem.join ml mr))
+  = Mem.intro_star q r ml mr
+  in
+  elim_star p r m;
+  Classical.forall_intro (Classical.move_requires proof);
+  Classical.forall_intro_2 (Classical.move_requires_2 intro)
+
+#push-options "--z3rlimit 20 --fuel 1 --ifuel 0"
+let change_slprop0 (#opened:inames) (p q:vprop) (vp:erased (t_of p)) (vq:erased (t_of q))
+  (proof:(m:mem) -> Lemma
+    (requires interp (hp_of p) m /\ sel_of p m == reveal vp)
+    (ensures interp (hp_of q) m /\ sel_of q m == reveal vq)
+  ) : repr unit false opened Unobservable p (fun _ -> q) (fun h -> h p == reveal vp) (fun _ _ h1 -> h1 q == reveal vq)
+  = fun frame ->
+      let m:full_mem = NMSTTotal.get () in
+      proof (core_mem m);
+      Classical.forall_intro (Classical.move_requires proof);
+      Mem.star_associative (hp_of p) frame (locks_invariant opened m);
+      intro_star p q (frame `Mem.star` locks_invariant opened m) vp vq m proof;
+      Mem.star_associative (hp_of q) frame (locks_invariant opened m)
+#pop-options
+
+let change_slprop p q vp vq l  = SteelSelGhost?.reflect (change_slprop0 p q vp vq l)
+
+let change_equal_slprop
+  p q
+= let m = get #p () in
+  let x : Ghost.erased (t_of p) = m p in
+  let y : Ghost.erased (t_of q) = Ghost.hide (Ghost.reveal x) in
+  change_slprop
+    p
+    q
+    x
+    y
+    (fun _ -> ())
+
+#push-options "--z3rlimit 20 --fuel 1 --ifuel 0"
+let change_slprop_20 (#opened:inames) (p q:vprop) (vq:erased (t_of q))
+  (proof:(m:mem) -> Lemma
+    (requires interp (hp_of p) m)
+    (ensures interp (hp_of q) m /\ sel_of q m == reveal vq)
+  ) : repr unit false opened Unobservable p (fun _ -> q)
+           (fun _ -> True) (fun _ _ h1 -> h1 q == reveal vq)
+  = fun frame ->
+      let m:full_mem = NMSTTotal.get () in
+      proof (core_mem m);
+      Classical.forall_intro (Classical.move_requires proof);
+      Mem.star_associative (hp_of p) frame (locks_invariant opened m);
+      intro_star p q (frame `Mem.star` locks_invariant opened m) (sel_of p m) vq m proof;
+      Mem.star_associative (hp_of q) frame (locks_invariant opened m)
+#pop-options
+
+let change_slprop_2 p q vq l = SteelSelGhost?.reflect (change_slprop_20 p q vq l)
+
+let change_slprop_rel0 (#opened:inames) (p q:vprop)
+  (rel : normal (t_of p) -> normal (t_of q) -> prop)
+  (proof:(m:mem) -> Lemma
+    (requires interp (hp_of p) m)
+    (ensures
+      interp (hp_of p) m /\
+      interp (hp_of q) m /\
+      rel (sel_of p m) (sel_of q m))
+  ) : repr unit false opened Unobservable p (fun _ -> q)
+           (fun _ -> True) (fun h0 _ h1 -> rel (h0 p) (h1 q))
+  = fun frame ->
+      let m:full_mem = NMSTTotal.get () in
+
+      proof (core_mem m);
+      let h0 = mk_rmem p (core_mem m) in
+      let h1 = mk_rmem q (core_mem m) in
+      reveal_mk_rmem p (core_mem m) p;
+      reveal_mk_rmem q (core_mem m) q;
+
+      Mem.star_associative (hp_of p) frame (locks_invariant opened m);
+      intro_star p q (frame `Mem.star` locks_invariant opened m) (sel_of p (core_mem m)) (sel_of q (core_mem m)) m proof;
+      Mem.star_associative (hp_of q) frame (locks_invariant opened m)
+
+let change_slprop_rel p q rel proof = SteelSelGhost?.reflect (change_slprop_rel0 p q rel proof)
+
+let change_slprop_rel_with_cond0 (#opened:inames) (p q:vprop)
+  (cond: t_of p -> prop)
+  (rel : (t_of p) -> (t_of q) -> prop)
+  (proof:(m:mem) -> Lemma
+    (requires interp (hp_of p) m /\ cond (sel_of p m))
+    (ensures
+      interp (hp_of p) m /\
+      interp (hp_of q) m /\
+      rel (sel_of p m) (sel_of q m))
+  ) : repr unit false opened Unobservable p (fun _ -> q)
+           (fun m -> cond (m p)) (fun h0 _ h1 -> rel (h0 p) (h1 q))
+  = fun frame ->
+      let m:full_mem = NMSTTotal.get () in
+
+      proof (core_mem m);
+      let h0 = mk_rmem p (core_mem m) in
+      let h1 = mk_rmem q (core_mem m) in
+      reveal_mk_rmem p (core_mem m) p;
+      reveal_mk_rmem q (core_mem m) q;
+
+      Mem.star_associative (hp_of p) frame (locks_invariant opened m);
+      intro_star p q (frame `Mem.star` locks_invariant opened m) (sel_of p (core_mem m)) (sel_of q (core_mem m)) m proof;
+      Mem.star_associative (hp_of q) frame (locks_invariant opened m)
+
+let change_slprop_rel_with_cond p q cond rel proof
+  = SteelSelGhost?.reflect (change_slprop_rel_with_cond0 p q cond rel proof)
+
+let extract_info0 (#opened:inames) (p:vprop) (vp:erased (normal (t_of p))) (fact:prop)
+  (l:(m:mem) -> Lemma
+    (requires interp (hp_of p) m /\ sel_of p m == reveal vp)
+    (ensures fact)
+  ) : repr unit false opened Unobservable p (fun _ -> p)
+      (fun h -> h p == reveal vp)
+      (fun h0 _ h1 -> normal (frame_equalities p h0 h1) /\ fact)
+  = fun frame ->
+      let m0:full_mem = NMSTTotal.get () in
+      let h0 = mk_rmem p (core_mem m0) in
+      lemma_frame_equalities_refl p h0;
+      l (core_mem m0)
+
+let extract_info p vp fact l = SteelSelGhost?.reflect (extract_info0 p vp fact l)
+
+let sladmit _ = SteelSelGhostF?.reflect (fun _ -> NMSTTotal.nmst_tot_admit ())
+
+let reveal_star0 (#opened:inames) (p1 p2:vprop)
+  : repr unit false opened Unobservable (p1 `star` p2) (fun _ -> p1 `star` p2)
+   (fun _ -> True)
+   (fun h0 _ h1 ->
+     h0 p1 == h1 p1 /\ h0 p2 == h1 p2 /\
+     h0 (p1 `star` p2) == (h0 p1, h0 p2) /\
+     h1 (p1 `star` p2) == (h1 p1, h1 p2)
+   )
+ = fun frame ->
+     let m:full_mem = NMSTTotal.get () in
+     let h0 = mk_rmem (p1 `star` p2) (core_mem m) in
+     reveal_mk_rmem (p1 `star` p2) m (p1 `star` p2);
+     reveal_mk_rmem (p1 `star` p2) m p1;
+     reveal_mk_rmem (p1 `star` p2) m p2
+
+let reveal_star p1 p2 = SteelSelGhost?.reflect (reveal_star0 p1 p2)
+
+let reveal_star_30 (#opened:inames) (p1 p2 p3:vprop)
+ : repr unit false opened Unobservable (p1 `star` p2 `star` p3) (fun _ -> p1 `star` p2 `star` p3)
+   (requires fun _ -> True)
+   (ensures fun h0 _ h1 ->
+     can_be_split (p1 `star` p2 `star` p3) p1 /\
+     can_be_split (p1 `star` p2 `star` p3) p2 /\
+     h0 p1 == h1 p1 /\ h0 p2 == h1 p2 /\ h0 p3 == h1 p3 /\
+     h0 (p1 `star` p2 `star` p3) == ((h0 p1, h0 p2), h0 p3) /\
+     h1 (p1 `star` p2 `star` p3) == ((h1 p1, h1 p2), h1 p3)
+   )
+ = fun frame ->
+     let m:full_mem = NMSTTotal.get () in
+     let h0 = mk_rmem (p1 `star` p2 `star` p3) (core_mem m) in
+     can_be_split_trans (p1 `star` p2 `star` p3) (p1 `star` p2) p1;
+     can_be_split_trans (p1 `star` p2 `star` p3) (p1 `star` p2) p2;
+     reveal_mk_rmem (p1 `star` p2 `star` p3) m (p1 `star` p2 `star` p3);
+     reveal_mk_rmem (p1 `star` p2 `star` p3) m (p1 `star` p2);
+     reveal_mk_rmem (p1 `star` p2 `star` p3) m p3
+
+let reveal_star_3 p1 p2 p3 = SteelSelGhost?.reflect (reveal_star_30 p1 p2 p3)
+
+let intro_vrefine v p =
+  let m = get () in
+  let x : Ghost.erased (t_of v) = Ghost.hide (m v) in
+  let x' : Ghost.erased (vrefine_t v p) = Ghost.hide (Ghost.reveal x) in
+  change_slprop
+    v
+    (vrefine v p)
+    x
+    x'
+    (fun m ->
+      interp_vrefine_hp v p m;
+      vrefine_sel_eq v p m
+    )
+
+let elim_vrefine v p =
+  let m = get () in
+  let x : Ghost.erased (vrefine_t v p) = Ghost.hide (m (vrefine v p)) in
+  let x' : Ghost.erased (t_of v) = Ghost.hide (Ghost.reveal x) in
+  change_slprop
+    (vrefine v p)
+    v
+    x
+    x'
+    (fun m ->
+      interp_vrefine_hp v p m;
+      vrefine_sel_eq v p m
+    )
+
+let vdep_cond
+  (v: vprop)
+  (q: vprop)
+  (p: (t_of v -> Tot vprop))
+  (x1: t_of (v `star` q))
+: Tot prop
+= q == p (fst x1)
+
+let vdep_rel
+  (v: vprop)
+  (q: vprop)
+  (p: (t_of v -> Tot vprop))
+  (x1: t_of (v `star` q))
+  (x2: (t_of (vdep v p)))
+: Tot prop
+=
+  q == p (fst x1) /\
+  dfst (x2 <: (dtuple2 (t_of v) (vdep_payload v p))) == fst x1 /\
+  dsnd (x2 <: (dtuple2 (t_of v) (vdep_payload v p))) == snd x1
+
+let intro_vdep_lemma
+  (v: vprop)
+  (q: vprop)
+  (p: (t_of v -> Tot vprop))
+  (m: mem)
+: Lemma
+  (requires (
+    interp (hp_of (v `star` q)) m /\
+    q == p (fst (sel_of (v `star` q) m))
+  ))
+  (ensures (
+    interp (hp_of (v `star` q)) m /\
+    interp (hp_of (vdep v p)) m /\
+    vdep_rel v q p (sel_of (v `star` q) m) (sel_of (vdep v p) m)
+  ))
+=
+  Mem.interp_star (hp_of v) (hp_of q) m;
+  interp_vdep_hp v p m;
+  vdep_sel_eq v p m
+
+let intro_vdep
+  v q p
+=
+  reveal_star v q;
+  change_slprop_rel_with_cond
+    (v `star` q)
+    (vdep v p)
+    (vdep_cond v q p)
+    (vdep_rel v q p)
+    (fun m -> intro_vdep_lemma v q p m)
+
+let vdep_cond_recip
+  (v: vprop)
+  (p: (t_of v -> Tot vprop))
+  (q: vprop)
+  (x2: t_of (vdep v p))
+: Tot prop
+= q == p (dfst (x2 <: dtuple2 (t_of v) (vdep_payload v p)))
+
+let vdep_rel_recip
+  (v: vprop)
+  (q: vprop)
+  (p: (t_of v -> Tot vprop))
+  (x2: (t_of (vdep v p)))
+  (x1: t_of (v `star` q))
+: Tot prop
+=
+  vdep_rel v q p x1 x2
+
+let elim_vdep_lemma
+  (v: vprop)
+  (q: vprop)
+  (p: (t_of v -> Tot vprop))
+  (m: mem)
+: Lemma
+  (requires (
+    interp (hp_of (vdep v p)) m /\
+    q == p (dfst (sel_of (vdep v p) m <: dtuple2 (t_of v) (vdep_payload v p)))
+  ))
+  (ensures (
+    interp (hp_of (v `star` q)) m /\
+    interp (hp_of (vdep v p)) m /\
+    vdep_rel v q p (sel_of (v `star` q) m) (sel_of (vdep v p) m)
+  ))
+=
+  Mem.interp_star (hp_of v) (hp_of q) m;
+  interp_vdep_hp v p m;
+  vdep_sel_eq v p m
+
+let elim_vdep0
+  (#opened:inames)
+  (v: vprop)
+  (p: (t_of v -> Tot vprop))
+  (q: vprop)
+: SteelSelGhost unit opened
+  (vdep v p)
+  (fun _ -> v `star` q)
+  (requires (fun h -> q == p (dfst (h (vdep v p)))))
+  (ensures (fun h _ h' ->
+      let fs = h' v in
+      let sn = h' q in
+      let x2 = h (vdep v p) in
+      q == p fs /\
+      dfst x2 == fs /\
+      dsnd x2 == sn
+  ))
+= change_slprop_rel_with_cond
+    (vdep v p)
+    (v `star` q)
+    (vdep_cond_recip v p q)
+    (vdep_rel_recip v q p)
+    (fun m -> elim_vdep_lemma v q p m);
+  reveal_star v q
+
+let elim_vdep
+  v p
+= let r = gget (vdep v p) in
+  let res = Ghost.hide (dfst #(t_of v) #(vdep_payload v p) (Ghost.reveal r)) in
+  elim_vdep0 v p (p (Ghost.reveal res));
+  res
+
+let intro_vrewrite
+  v #t f
+=
+  let m = get () in
+  let x : Ghost.erased (t_of v) = Ghost.hide (m v) in
+  let x' : Ghost.erased t = Ghost.hide (f (Ghost.reveal x)) in
+  change_slprop
+    v
+    (vrewrite v f)
+    x
+    x'
+    (fun m ->
+      vrewrite_sel_eq v f m
+    )
+
+let elim_vrewrite
+  v #t f
+=
+  change_slprop_rel
+    (vrewrite v f)
+    v
+    (fun y x -> y == f x)
+    (fun m -> vrewrite_sel_eq v f m)
